clight_examples/xorlist/xorlist1.v
@@ -14,10 +14,10 @@ Set Implicit Arguments.
 
 Section PROP.
 
-  Context `{@GRA.inG memcntRA Σ}.
-  Context `{@GRA.inG memphyRA Σ}.
-  Context `{@GRA.inG memhdRA Σ}.
-  Context `{@GRA.inG memidRA Σ}.
+  Context `{@GRA.inG pointstoRA Σ}.
+  Context `{@GRA.inG allocatedRA Σ}.
+  Context `{@GRA.inG blocksizeRA Σ}.
+  Context `{@GRA.inG blockaddressRA Σ}.
 
   Definition vlist_add (x: val) (l : list val) (at_tail: val) : list val :=
     if Val.eq at_tail Vzero then x :: l else snoc l x.
@@ -26,13 +26,19 @@ Section PROP.
     if Val.eq from_tail Vzero then (hd default l, tl l)
     else (last l default, removelast l).
 
-  Definition vnth (index: val) (l: list val) (from_tail: val) (default: val) : val :=
+  Definition check_inbound (l: list val) (from_tail: val) (index: val) : option nat :=
     match index with
-    | Vint i => if Val.eq from_tail Vzero then nth (Z.to_nat (Int.unsigned i)) l default
-                else nth (List.length l - Z.to_nat (Int.unsigned i) - 1) l default
-    | Vlong i => if Val.eq from_tail Vzero then nth (Z.to_nat (Int64.unsigned i)) l default
-                 else nth (List.length l - Z.to_nat (Int64.unsigned i) - 1) l default
-    | _ => Vundef
+    | Vint i =>
+      if negb (Coqlib.zle 0 (Int.unsigned i) && Coqlib.zlt (Int.unsigned i) (Z.of_nat (List.length l)))
+      then None
+      else if Val.eq Vzero from_tail then Some (Z.to_nat (Int.unsigned i))
+           else Some (List.length l - Z.to_nat (Int.unsigned i))
+    | Vlong i => 
+      if negb (Coqlib.zle 0 (Int64.unsigned i) && Coqlib.zlt (Int64.unsigned i) (Z.of_nat (List.length l)))
+      then None
+      else if Val.eq Vzero from_tail then Some (Z.to_nat (Int64.unsigned i))
+           else Some (List.length l - Z.to_nat (Int64.unsigned i))
+    | _ => None
     end.
 
      (* is_xorlist represents the figure below    *)
@@ -41,37 +47,203 @@ Section PROP.
      (*     v                                 v   *)
      (* xs  - - - - - - - - - - - - - - - - - -   *)
 
-  
-  Fixpoint _is_xorlist (hd_prev : val) (hd : val) (tl : val) (xs : list val) {struct xs} : iProp :=
+  Fixpoint frag_xorlist (q: Qp) (p_hd_prev p_hd p_tl p_tl_next: val) (xs : list val) {struct xs} : iProp :=
     match xs with
-    | [] => ⌜hd_prev = Vnullptr /\ hd = Vnullptr /\ tl = Vnullptr⌝
-    | h :: t => 
-      if Val.eq Vnullptr hd_prev then
-
-      else ∃ b_prev ofs_prev hd_next b_next ofs_next i_hd_prev i_hd_next item,
-                hd_prev ~~ (b_prev, ofs_prev)
-                ** b_prev ↱1# (8, Dynamic, Some i_hd_prev)
-                ** hd_next ~~ (b_next, ofs_next)
-                ** b_next ↱1# (8, Dynamic, Some i_hd_next)
-                ** hd ⊢1#> (encode_val Mint64 item
-                            ++ encode_val Mptr (Vptrofs (Ptrofs.repr (Z.lxor i_hd_prev i_hd_next))))
-                ** _is_xorlist hd hd_next tl t
+    | [] => ⌜p_hd_prev = p_tl /\ p_hd = p_tl_next⌝
+    | Vlong a :: xs' =>
+      if Val.eq Vnullptr p_hd_prev
+      then
+        ∃ p_next m_hd m_next i_next ofs_next tg_next,
+          p_hd ↦m_hd#q≻ (encode_val Mint64 (Vlong a) ++ encode_val Mptr (Vptrofs (Ptrofs.repr i_next)))
+          ** (if Z.eqb i_next 0 then ⌜p_next = Vnullptr⌝
+             else (p_next ⊨m_next# ofs_next
+                  ** live_ q # (m_next, tg_next) 
+                  ** p_next (≃_ m_next) i_next))
+          ** frag_xorlist q p_hd p_next p_tl p_tl_next xs'
+      else
+        ∃ p_next m_prev m_hd m_next i_prev i_key ofs_next tg_next,
+          p_hd ↦m_hd#q≻ (encode_val Mint64 (Vlong a) ++ encode_val Mptr (Vptrofs (Ptrofs.repr i_key)))
+          ** p_hd_prev (≃_ m_prev) i_prev
+          ** (if Z.eqb (Z.lxor i_prev i_key) 0 then ⌜p_next = Vnullptr⌝
+             else (p_next ⊨m_next# ofs_next)
+                  ** live_ q # (m_next, tg_next) 
+                  ** p_next (≃_ m_next) (Z.lxor i_prev i_key))
+          ** frag_xorlist q p_hd p_next p_tl p_tl_next xs'
+    | _ => False
     end%I.
 
-  Definition is_xorlist := _is_xorlist Vnullptr. 
+  Definition full_xorlist q p_hd p_tl xs : iProp := 
+    frag_xorlist q Vnullptr p_hd p_tl Vnullptr xs.
+
+  Lemma real_pointer_notnull'
+      vaddr m ofs
+    :
+      vaddr ⊨m# ofs ⊢ ⌜Coqlib.proj_sumbool (Val.eq Vnullptr vaddr) = false⌝.
+  Proof.
+  Admitted.
+
+  Lemma points_to_notnull
+      vaddr m q mvs
+    :
+      vaddr ↦m#q≻ mvs ⊢ ⌜Coqlib.proj_sumbool (Val.eq Vnullptr vaddr) = false⌝.
+  Proof.
+  Admitted.
+
+
+  Example xorlist_example1 p1 p2 p3 m1 m2 m3 i1 i2 i3 ofs3 tg3 ofs2 tg2:
+  p1 ↦m1#1≻ (encode_val Mint64 (Vlong Int64.one) ++ encode_val Mint64 (Vlong (Int64.repr i2)))
+  ** p1 (≃_ m1) i1
+  ** p2 ↦m2#1≻ (encode_val Mint64 (Vlong Int64.one) ++ encode_val Mint64 (Vptrofs (Ptrofs.repr (Z.lxor i1 i3))))
+  ** p2 ⊨m2# ofs2
+  ** live_ 1# (m2, tg2)
+  ** p2 (≃_ m2) i2
+  ** p3 ↦m3#1≻ (encode_val Mint64 (Vlong Int64.one) ++ encode_val Mint64 (Vlong (Int64.repr i2)))
+  ** p3 ⊨m3# ofs3
+  ** live_ 1# (m3, tg3)
+  ** p3 (≃_ m3) i3
+  ⊢ full_xorlist 1 p1 p3 [Vlong Int64.one;Vlong Int64.one;Vlong Int64.one].
+  Proof.
+  Admitted.
+    (* iIntros "[[[[[[[i j] h] b] c] d] e] f]".
+    unfold full_xorlist. ss. des_ifs_safe.
+    iExists _,_,_,_,_,_. unfold Vptrofs in *.
+    destruct Archi.ptr64 eqn: X; clarify.
+    ss. unfold Mptr in *.
+    destruct Archi.ptr64 eqn: X'; clarify.
+    unfold Ptrofs.to_int64 in *.
+    iPoseProof (points_to_notnull with "i") as "%".
+    iPoseProof (captured_pointer_notnull with "c") as "%".
+    iPoseProof (capture_dup with "c") as "[c c']".
+    iSplitL "i b c".
+    { instantiate (1:= i2). 
+      rewrite (Int64.unsigned_repr (Ptrofs.unsigned _)).
+      2:{ change Int64.max_unsigned with Ptrofs.max_unsigned.
+          apply Ptrofs.unsigned_range_2. }
+      iFrame. 
+      instantiate (2:=p2).
+      destruct (i2 =? 0)%Z eqn:E.
+      { apply Z.eqb_eq in E. clarify. }
+      iFrame. }
+    iPoseProof (captured_pointer_notnull with "f") as "%".
+    destruct (Val.eq _ _); ss; clarify.
+    iExists _,_,_,_,_,_,_,_.
+    iPoseProof (points_to_notnull with "h") as "%".
+    iSplitL "h e f j".
+    { instantiate (1:=(Z.lxor i1 i3)).
+      instantiate (3:=p3).
+      rewrite (Int64.unsigned_repr (Ptrofs.unsigned _)).
+      2:{ change Int64.max_unsigned with Ptrofs.max_unsigned.
+          apply Ptrofs.unsigned_range_2. }
+      rewrite <- Z.lxor_assoc. rewrite Z.lxor_nilpotent.
+      rewrite Z.lxor_0_l.
+      destruct (i3 =? 0)%Z eqn: E'.
+      { apply Z.eqb_eq in E'. clarify. }
+      iFrame. }
+    destruct (Val.eq _ _); ss; clarify.
+    iExists _,_,_,_,_,_,_,_.
+    instantiate (2:=i2).
+    rewrite (Int64.unsigned_repr (Ptrofs.unsigned _)).
+    2:{ change Int64.max_unsigned with Ptrofs.max_unsigned.
+        apply Ptrofs.unsigned_range_2. }
+    iFrame. iSplit; et. rewrite Z.lxor_nilpotent. ss.
+  Unshelve. all: et.
+  Qed. *)
+
+  Example xorlist_example2 p2 m2:
+  p2 ↦m2#1≻ (encode_val Mint64 (Vlong Int64.one) ++ encode_val Mint64 (Vptrofs Ptrofs.zero))
+  ⊢ full_xorlist 1 p2 p2 [Vlong Int64.one].
+  Proof.
+    iIntros "d".
+    unfold full_xorlist. ss.
+    destruct (Val.eq Vnullptr _); clarify.
+    iExists _,_,_,_,_,_. iFrame. ss.
+  Unshelve.
+  - exact m2.
+  - exact 0.
+  - exact Local.
+  Qed.
+    
+  Lemma split_xorlist q p_hd_prev p_hd p_tl p_tl_next xs0 xs1
+    : frag_xorlist q p_hd_prev p_hd p_tl p_tl_next (xs0 ++ xs1)
+      ⊢ ∃ mid mid_next, frag_xorlist q p_hd_prev p_hd mid mid_next xs0 ** frag_xorlist q mid mid_next p_tl p_tl_next xs1.
+  Proof.
+    (* revert q p_hd_prev p_hd p_tl p_tl_next xs1.
+    induction xs0; i; ss.
+    - iIntros "A". iExists _,_. iSplit; et.
+    - iIntros "A". des_ifs.
+      + iDestruct "A" as (p_next m_hd m_next i_next ofs_next tg_next) "[PTO NXT]".
+        iDestruct "PTO" as "[PTO RES]". clarify.
+        iPoseProof (IHxs0 with "NXT") as (mid mid_next) "[NXT0 NXT1]".
+        des_ifs.
+        * apply Z.eqb_eq in Heq. clarify.
+          iDestruct "RES" as "%". clarify.
+          iExists _,_. iFrame.
+          iExists _,_,_,_,_,_. iFrame. ss.
+        * iDestruct "RES" as "[NXT_ALIVE NXT_CAP]". clarify.
+          iExists _,_. iFrame.
+          iExists _,_,_,_,_,_. iFrame. rewrite Heq.
+          iFrame.
+      + iDestruct "A" as (p_next m_prev m_hd m_next i_prev i_key ofs_next tg_next) "[PTO NXT]".
+        iDestruct "PTO" as "[[PTO CAP_PREV] RES]".
+        iPoseProof (IHxs0 with "NXT") as (mid mid_next) "[NXT0 NXT1]".
+        des_ifs.
+        * iDestruct "RES" as "%". apply Z.eqb_eq in Heq. clarify.
+          iExists _,_. iFrame.
+          iExists _,_,_,_,_,_,_,_. iFrame. rewrite Heq.
+          ss.
+        * iDestruct "RES" as "[NXT_ALIVE NXT_CAP]".
+          iExists _,_. iFrame.
+          iExists _,_,_,_,_,_,_,_. iFrame. rewrite Heq.
+          iFrame.
+  Unshelve. all: et.
+  Qed. *)
+  Admitted.
+
+  Lemma concat_xorlist q p_hd_prev p_hd p_tl p_tl_next mid mid_next xs0 xs1
+    : frag_xorlist q p_hd_prev p_hd mid mid_next xs0 ** frag_xorlist q mid mid_next p_tl p_tl_next xs1
+      ⊢ frag_xorlist q p_hd_prev p_hd p_tl p_tl_next (xs0 ++ xs1).
+  Proof.
+    (* revert q p_hd_prev p_hd p_tl p_tl_next mid mid_next xs1.
+    induction xs0; i; ss.
+    - iIntros "[% A]". des. clarify.
+    - iIntros "A". des_ifs; try solve [iDestruct "A" as "[% A]"; clarify].
+      + iDestruct "A" as "[PTO NXT1]". 
+        iDestruct "PTO" as (p_next m_hd m_next i_next ofs_next tg_next) "[[PTO RES] NXT0]".
+        clarify. iCombine "NXT0 NXT1" as "NXT".
+        iPoseProof (IHxs0 with "NXT") as "NXT".
+        des_ifs.
+        * apply Z.eqb_eq in Heq. clarify.
+          iDestruct "RES" as "%". clarify.
+          iExists _,_,_,_,_,_. iFrame. ss.
+        * iDestruct "RES" as "[NXT_ALIVE NXT_CAP]".
+          iExists _,_,_,_,_,_. iFrame. rewrite Heq.
+          iFrame.
+      + iDestruct "A" as "[PTO NXT1]". 
+        iDestruct "PTO" as (p_next m_prev m_hd m_next i_prev i_key ofs_next tg_next) "[[[PTO CAP_PREV] RES] NXT]".
+        clarify. iCombine "NXT NXT1" as "NXT".
+        iPoseProof (IHxs0 with "NXT") as "NXT".
+        des_ifs.
+        * iDestruct "RES" as "%". apply Z.eqb_eq in Heq. clarify.
+          iExists _,_,_,_,_,_,_,_. iFrame. rewrite Heq.
+          ss.
+        * iDestruct "RES" as "[NXT_ALIVE NXT_CAP]".
+          iExists _,_,_,_,_,_,_,_. iFrame. rewrite Heq.
+          iFrame.
+  Unshelve. all: et.
+  Qed. *)
+  Admitted.
 
 End PROP.
 
-
 Section SPEC.
 
-  Context `{@GRA.inG memcntRA Σ}.
-  Context `{@GRA.inG memphyRA Σ}.
-  Context `{@GRA.inG memhdRA Σ}.
-  Context `{@GRA.inG memidRA Σ}.
+  Context `{@GRA.inG pointstoRA Σ}.
+  Context `{@GRA.inG allocatedRA Σ}.
+  Context `{@GRA.inG blocksizeRA Σ}.
+  Context `{@GRA.inG blockaddressRA Σ}.
 
   (* The function only requires resource needed by capture *)
-  Definition encrypt_spec : fspec :=
+  (* Definition encrypt_spec : fspec :=
     (mk_simple
       (fun '(left_ptr, right_ptr, b1, b2, sz1, sz2, tag1, tag2, q1, q2) => (
             (ord_pure 1%nat),
@@ -84,20 +256,69 @@ Section SPEC.
                           ** b1 ↱q1# (sz1, tag1, Some i1)
                           ** b2 ↱q2# (sz2, tag2, Some i2))
 
-    )))%I.
+    )))%I. *)
+  Definition encrypt_hoare1 : _ -> ord * (Any.t -> iProp) * (Any.t -> iProp) :=
+      fun '(left_ptr, right_ptr, m_l, m_r, tg_l, tg_r, q_l, q_r) => (
+            (ord_pure 1%nat),
+            (fun varg => ∃ ofs_l ofs_r, ⌜varg = [left_ptr; right_ptr]↑⌝
+                         ** left_ptr ⊨m_l# ofs_l
+                         ** right_ptr ⊨m_r# ofs_r
+                         ** live_ q_l# (m_l, tg_l)
+                         ** live_ q_r# (m_r, tg_r)),
+            (fun vret => ∃ i_l i_r, ⌜vret = (Vptrofs (Ptrofs.repr (Z.lxor i_l i_r)))↑⌝
+                         ** left_ptr (≃_ m_l) i_l
+                         ** right_ptr (≃_ m_r) i_r
+                         ** live_ q_l# (m_l, tg_l)
+                         ** live_ q_r# (m_r, tg_r)))%I.
 
-  (* The function requires resource needed by capture *)
-  Definition decrypt_spec : fspec :=
-    (mk_simple
-      (fun '(i1, ptr, b, sz, tag, q) => (
+  Definition encrypt_hoare2 : _ -> ord * (Any.t -> iProp) * (Any.t -> iProp) :=
+      fun '(left_ptr, m_l, tg_l, q_l) => (
+            (ord_pure 1%nat),
+            (fun varg => ∃ ofs_l, ⌜varg = [left_ptr; Vnullptr]↑⌝
+                         ** left_ptr ⊨m_l# ofs_l
+                         ** live_ q_l# (m_l, tg_l)),
+            (fun vret => ∃ i_l, ⌜vret = (Vptrofs (Ptrofs.repr i_l))↑⌝
+                         ** left_ptr (≃_ m_l) i_l
+                         ** live_ q_l# (m_l, tg_l)))%I.
+
+  Definition encrypt_hoare3 : _ -> ord * (Any.t -> iProp) * (Any.t -> iProp) :=
+      fun '(right_ptr, m_r, tg_r, q_r) => (
+            (ord_pure 1%nat),
+            (fun varg => ∃ ofs_r, ⌜varg = [Vnullptr; right_ptr]↑⌝
+                         ** right_ptr ⊨m_r# ofs_r
+                         ** live_ q_r# (m_r, tg_r)),
+            (fun vret => ∃ i_r, ⌜vret = (Vptrofs (Ptrofs.repr i_r))↑⌝
+                         ** right_ptr (≃_ m_r) i_r
+                         ** live_ q_r# (m_r, tg_r)))%I.
+  
+  Definition encrypt_spec :=
+    mk_simple (
+      encrypt_hoare1
+      @ encrypt_hoare2
+      @ encrypt_hoare3
+    ).
+
+  Definition decrypt_hoare1 : _ -> ord * (Any.t -> iProp) * (Any.t -> iProp) :=
+      fun '(i_key, ptr, m, q, tg) => (
         (ord_pure 1%nat),
-        (fun varg => ∃ ofs opt key, ⌜varg = [key; ptr]↑ /\ key = Vptrofs i1⌝
-                     ** ptr ⊸ (b, ofs)
-                     ** b ↱q# (sz, tag, opt)),
-        (fun vret => ∃ i2, ⌜vret = (Vptrofs (Ptrofs.xor i1 (Ptrofs.repr i2)))↑⌝
-                     ** b ↱q# (sz, tag, Some i2))
+        (fun varg => ∃ key ofs, ⌜varg = [key; ptr]↑ /\ key = Vptrofs i_key⌝
+                     ** ptr ⊨m# ofs
+                     ** live_ q# (m, tg)),
+        (fun vret => ∃ i_ptr, ⌜vret = (Vptrofs (Ptrofs.xor i_key (Ptrofs.repr i_ptr)))↑⌝
+                     ** ptr (≃_m) i_ptr
+                     ** live_ q# (m, tg)))%I.
                      
-    )))%I.
+  Definition decrypt_hoare2 : _ -> ord * (Any.t -> iProp) * (Any.t -> iProp) :=
+      fun '(i_key) => (
+        (ord_pure 1%nat),
+        (fun varg => ∃ key, ⌜varg = [key; Vnullptr]↑ /\ key = Vptrofs i_key⌝),
+        (fun vret => ⌜vret = (Vptrofs i_key)↑⌝))%I.
+  
+  Definition decrypt_spec : fspec :=
+    mk_simple (
+      decrypt_hoare1
+      @ decrypt_hoare2
+    ).
 
   (* {hd_handler |-> hd  /\ tl_handler |-> tl /\ is_xorlist hd tl xs}
      void add(node** hd_handler, node** tl_handler, long item, bool at_tail)
@@ -110,19 +331,18 @@ Section SPEC.
 
   Definition add_spec : fspec :=
     (mk_simple
-      (fun '(hd_handler, tl_handler, item, at_tail, xs) => (
+      (fun '(hd_handler, tl_handler, m_h, m_t, item, at_tail, xs) => (
         (ord_pure 2%nat),
         (fun varg => ∃ hd_old tl_old,
-                     ⌜varg = [hd_handler; tl_handler; item; at_tail]↑⌝
-                     (* item should be vlong *)
-                     ** hd_handler ⊢1#> encode_val Mptr hd_old
-                     ** tl_handler ⊢1#> encode_val Mptr tl_old
-                     ** is_xorlist hd_old tl_old xs),
+                     ⌜varg = [hd_handler; tl_handler; Vlong item; Vint at_tail]↑⌝
+                     ** hd_handler ↦m_h#1≻ encode_val Mptr hd_old
+                     ** tl_handler ↦m_t#1≻ encode_val Mptr tl_old
+                     ** full_xorlist 1 hd_old tl_old xs),
         (fun vret => ∃ hd_new tl_new,
                      ⌜vret = Vundef↑⌝
-                     ** hd_handler ⊢1#> encode_val Mptr hd_new
-                     ** tl_handler ⊢1#> encode_val Mptr tl_new
-                     ** is_xorlist hd_new tl_new (vlist_add item xs at_tail))
+                     ** hd_handler ↦m_h#1≻ encode_val Mptr hd_new
+                     ** tl_handler ↦m_t#1≻ encode_val Mptr tl_new
+                     ** full_xorlist 1 hd_new tl_new (vlist_add (Vlong item) xs (Vint at_tail)))
     )))%I.
 
   (* {hd_handler |-> hd  /\ tl_handler |-> tl /\ is_xorlist hd tl xs}
@@ -135,40 +355,33 @@ Section SPEC.
      } *)
   Definition delete_spec : fspec :=
     (mk_simple
-      (fun '(hd_handler, tl_handler, from_tail, xs) => (
+      (fun '(hd_handler, tl_handler, m_h, m_t, from_tail, xs) => (
         (ord_pure 2%nat),
-        (fun varg => ∃ hd_old tl_old, ⌜varg = [hd_handler; tl_handler; from_tail]↑⌝
-                     ** hd_handler ⊢1#> encode_val Mptr hd_old
-                     ** tl_handler ⊢1#> encode_val Mptr tl_old
-                     ** is_xorlist hd_old tl_old xs),
-        (fun vret => let '(item, xs') := vlist_delete xs from_tail (Vlong Int64.zero) in
+        (fun varg => ∃ hd_old tl_old, ⌜varg = [hd_handler; tl_handler; Vint from_tail]↑⌝
+                     ** hd_handler ↦m_h#1≻ encode_val Mptr hd_old
+                     ** tl_handler ↦m_t#1≻ encode_val Mptr tl_old
+                     ** full_xorlist 1 hd_old tl_old xs),
+        (fun vret => let '(item, xs') := vlist_delete xs (Vint from_tail) (Vlong Int64.zero) in
                      ∃ hd_new tl_new, ⌜vret = item↑⌝
-                     ** hd_handler ⊢1#> encode_val Mptr hd_new
-                     ** tl_handler ⊢1#> encode_val Mptr tl_new
-                     ** is_xorlist hd_new tl_new xs')
+                     ** hd_handler ↦m_h#1≻ encode_val Mptr hd_new
+                     ** tl_handler ↦m_t#1≻ encode_val Mptr tl_new
+                     ** full_xorlist 1 hd_new tl_new xs')
     )))%I.
-
-  (* {is_xorlist hd tl xs}
-     node* search(node* hd, size_t index)
-     {r. r = nth index xs 0 /\ is_xorlist hd tl xs} *)
 
   Definition search_spec : fspec :=
     (mk_simple
-      (fun '(hd_handler, tl_handler, from_tail, index, xs) => (
+      (fun '(hd_handler, tl_handler, from_tail, index, idx, xs, m_h, m_t, q, q_h, q_t) => (
         (ord_pure 2%nat),
-        (fun varg => ∃ hd tl,
-                     ⌜varg = [hd_handler; tl_handler; from_tail; index]↑⌝
-                     ** hd_handler ⊢1#> encode_val Mptr hd
-                     ** tl_handler ⊢1#> encode_val Mptr tl
-                     ** is_xorlist hd tl xs),
-        (fun vret => let item := vnth index xs from_tail (Vlong Int64.zero) in
-                     ∃ hd tl node link b ofs q opti, ⌜vret = node↑ /\ (q < 1)%Qp⌝
-                     ** hd_handler ⊢1#> encode_val Mptr hd
-                     ** tl_handler ⊢1#> encode_val Mptr tl
-                     ** node ⊢q#> ((encode_val Mint64 item) ++ (encode_val Mptr link))
-                     ** node ⊸ (b, ofs)
-                     ** b ↱q# (8, Dynamic, opti)
-                     ** is_xorlist hd tl xs)
+        (fun varg => ∃ hd tl, ⌜varg = [hd_handler; tl_handler; Vint from_tail; Vlong index]↑
+                     /\ check_inbound xs (Vint from_tail) (Vlong index) = Some idx⌝
+                     ** hd_handler ↦m_h#q_h≻ encode_val Mptr hd
+                     ** tl_handler ↦m_t#q_t≻ encode_val Mptr tl
+                     ** full_xorlist q hd tl xs),
+        (fun vret => ∃ hd tl mid mid_prev, ⌜vret = mid↑⌝
+                     ** hd_handler ↦m_h#q_h≻ encode_val Mptr hd
+                     ** tl_handler ↦m_t#q_t≻ encode_val Mptr tl
+                     ** frag_xorlist q mid_prev mid tl Vnullptr (drop idx xs)
+                     ** frag_xorlist q Vnullptr hd mid_prev mid (firstn idx xs))
     )))%I.
 
   (* sealed *)
@@ -188,10 +401,10 @@ Require Import xorlist0.
 
 Section SMOD.
 
-  Context `{@GRA.inG memcntRA Σ}.
-  Context `{@GRA.inG memphyRA Σ}.
-  Context `{@GRA.inG memidRA Σ}.
-  Context `{@GRA.inG memhdRA Σ}.
+  Context `{@GRA.inG pointstoRA Σ}.
+  Context `{@GRA.inG allocatedRA Σ}.
+  Context `{@GRA.inG blocksizeRA Σ}.
+  Context `{@GRA.inG blockaddressRA Σ}.
 
   Definition xorSbtb: list (gname * fspecbody) :=
     [("encrypt",  mk_pure encrypt_spec);
