clightdm/proofmode/CIProofMode.v
@@ -34,10 +34,12 @@ Section MEM.
         (inv_with le I w0 st_src st_tgt
                   ** 
                   (∀ st_src st_tgt vaddr m,
-                      ((inv_with le I w0 st_src st_tgt) ** (⌜m.(sz) = Z.of_nat n⌝ ** vaddr ↦m#1≻ List.repeat Undef n ** vaddr ⊨m#1≖ (0, Local))) -* isim le I mn stb o (g, g, true, true) Q (Some fuel1) (st_src, itr_src) (st_tgt, ktr_tgt (m.(blk)))))
+                      ((inv_with le I w0 st_src st_tgt)
+                        ** (⌜m.(sz) = Z.of_nat n /\ n ≤ Z.to_nat Ptrofs.max_unsigned⌝ ** vaddr ↦m#1≻ List.repeat Undef n ** vaddr ⊨m# 0 ** live_ 1# (m, Local)))
+                      -* isim le I mn stb o (g, g, true, true) Q (Some fuel1) (st_src, itr_src) (st_tgt, ktr_tgt (m.(blk)))))
         (isim le I mn stb o (r, g, f_src, f_tgt) Q (Some fuel0) (st_src, itr_src) (st_tgt, ccallU "salloc" n >>= ktr_tgt)).
   Proof.
-    iIntros "[H0 H1]". iApply isim_ccallU_pure; et.
+    (* iIntros "[H0 H1]". iApply isim_ccallU_pure; et.
     { eapply fn_has_spec_in_stb; et.
       { eapply STBINCL. stb_tac. ss. }
       { ss. }
@@ -52,7 +54,8 @@ Section MEM.
     des. clarify.
     iExists _. iSplit; ss; et.
     iApply "H1". iFrame. 
-  Qed.
+  Qed. *)
+  Admitted.
 
   Lemma isim_ccallU_sfree
         o stb w0 fuel1
@@ -67,13 +70,13 @@ Section MEM.
     :
       bi_entails
         (inv_with le I w0 st_src st_tgt
-                  ** (∃ m mvl vaddr, vaddr ↦m#1≻ mvl ** vaddr ⊨m#1≖ (0, Local) ** ⌜m.(blk) = b /\ m.(sz) = size /\ Z.of_nat (List.length mvl) = m.(sz)⌝)
+                  ** (∃ m mvl vaddr, vaddr ↦m#1≻ mvl ** vaddr ⊨m# 0 ** live_ 1# (m, Local) ** ⌜m.(blk) = b /\ m.(sz) = size /\ Z.of_nat (List.length mvl) = m.(sz)⌝)
                   **
                   (∀ st_src st_tgt,
                       ((inv_with le I w0 st_src st_tgt)) -* isim le I mn stb o (g, g, true, true) Q (Some fuel1) (st_src, itr_src) (st_tgt, ktr_tgt tt)))
         (isim le I mn stb o (r, g, f_src, f_tgt) Q (Some fuel0) (st_src, itr_src) (st_tgt, ccallU "sfree" (b, size) >>= ktr_tgt)).
   Proof.
-    iIntros "[H0 H1]". iApply isim_ccallU_pure; et.
+    (* iIntros "[H0 H1]". iApply isim_ccallU_pure; et.
     { eapply fn_has_spec_in_stb; et.
       { eapply STBINCL. stb_tac. ss. }
       { ss. des_ifs. }
@@ -90,7 +93,8 @@ Section MEM.
     des. clarify.
     iExists _. iSplit; ss.
     iApply "H1". iFrame. 
-  Qed.
+  Qed. *)
+  Admitted.
 
   Lemma isim_ccallU_load
         o stb w0 fuel1
@@ -105,13 +109,13 @@ Section MEM.
     :
       bi_entails
         (inv_with le I w0 st_src st_tgt
-                  ** (vaddr ↦m#q≻ mvs ** ⌜List.length mvs = size_chunk_nat chunk⌝)
+                  ** (∃ ofs, vaddr ↦m#q≻ mvs ** vaddr ⊨m# ofs ** ⌜List.length mvs = size_chunk_nat chunk /\ ((size_chunk chunk) | ofs)%Z⌝)
                   **
                   (∀ st_src st_tgt,
                       ((inv_with le I w0 st_src st_tgt) ** (vaddr ↦m#q≻ mvs)) -* isim le I mn stb o (g, g, true, true) Q (Some fuel1) (st_src, itr_src) (st_tgt, ktr_tgt (decode_val chunk mvs))))
         (isim le I mn stb o (r, g, f_src, f_tgt) Q (Some fuel0) (st_src, itr_src) (st_tgt, ccallU "load" (chunk, vaddr) >>= ktr_tgt)).
   Proof.
-    iIntros "[H0 H1]". iApply isim_ccallU_pure; et.
+    (* iIntros "[H0 H1]". iApply isim_ccallU_pure; et.
     { eapply fn_has_spec_in_stb; et.
       { eapply STBINCL. stb_tac. ss. }
       { ss. des_ifs_safe. destruct p. ss. }
@@ -126,7 +130,8 @@ Section MEM.
     des. clarify.
     iExists _. iSplit; ss.
     iApply "H1". iFrame. 
-  Qed.
+  Qed. *)
+  Admitted.
 
   Lemma isim_ccallU_store
         o stb w0 fuel1
@@ -141,13 +146,15 @@ Section MEM.
     :
       bi_entails
         (inv_with le I w0 st_src st_tgt
-                  ** (∃ mvs_old, ⌜length mvs_old = size_chunk_nat chunk⌝ ** vaddr ↦m#1≻ mvs_old)
+                  ** (∃ mvs_old ofs, ⌜length mvs_old = size_chunk_nat chunk /\ ((size_chunk chunk) | ofs)%Z⌝
+                     ** vaddr ↦m#1≻ mvs_old
+                     ** vaddr ⊨m# ofs)
                   **
                   (∀ st_src st_tgt,
                       ((inv_with le I w0 st_src st_tgt) ** (vaddr ↦m#1≻ (encode_val chunk v_new))) -* isim le I mn stb o (g, g, true, true) Q (Some fuel1) (st_src, itr_src) (st_tgt, ktr_tgt tt)))
         (isim le I mn stb o (r, g, f_src, f_tgt) Q (Some fuel0) (st_src, itr_src) (st_tgt, ccallU "store" (chunk, vaddr, v_new) >>= ktr_tgt)).
   Proof.
-    iIntros "[H0 H1]". iApply isim_ccallU_pure; et.
+    (* iIntros "[H0 H1]". iApply isim_ccallU_pure; et.
     { eapply fn_has_spec_in_stb; et.
       { eapply STBINCL. stb_tac. ss. }
       { ss. des_ifs_safe. destruct p0. ss. }
@@ -163,7 +170,8 @@ Section MEM.
     des. clarify.
     iExists _. iSplit; ss.
     iApply "H1". iFrame. 
-  Qed.
+  Qed. *)
+  Admitted.
 
   Lemma isim_ccallU_cmp_ptr0
         o stb w0 fuel1
@@ -208,13 +216,13 @@ Section MEM.
     :
       bi_entails
         (inv_with le I w0 st_src st_tgt
-                  ** (⌜weak_valid m ofs⌝ ** vaddr ⊨m#q≖ (ofs, tg))
+                  ** (weak_valid m vaddr ofs ** live_ q# (m, tg))
                   **
                   (∀ st_src st_tgt,
-                      ((inv_with le I w0 st_src st_tgt) ** (vaddr ⊨m#q≖ (ofs, tg))) -* isim le I mn stb o (g, g, true, true) Q (Some fuel1) (st_src, itr_src) (st_tgt, ktr_tgt false)))
+                      ((inv_with le I w0 st_src st_tgt) ** (live_ q# (m, tg))) -* isim le I mn stb o (g, g, true, true) Q (Some fuel1) (st_src, itr_src) (st_tgt, ktr_tgt false)))
         (isim le I mn stb o (r, g, f_src, f_tgt) Q (Some fuel0) (st_src, itr_src) (st_tgt, ccallU "cmp_ptr" (Ceq, Vnullptr, vaddr) >>= ktr_tgt)).
   Proof.
-    iIntros "[[H0 [% H2]] H1]". iApply isim_ccallU_pure; et.
+    (* iIntros "[[H0 [% H2]] H1]". iApply isim_ccallU_pure; et.
     { eapply fn_has_spec_in_stb; et.
       { eapply STBINCL. stb_tac. ss. }
       { ss. instantiate(1:=inr (inl _)).
@@ -228,14 +236,15 @@ Section MEM.
     - iIntros (st_src0 st_tgt0 ret_src ret_tgt) "H0".
       iDestruct "H0" as "[INV [[% AL] %]]".
       rewrite H4. iExists _. iSplit; et; iApply "H1"; iFrame.
-  Qed.
+  Qed. *)
+  Admitted.
 
   Lemma isim_ccallU_cmp_ptr2
         o stb w0 fuel1
         R_src R_tgt
         (Q: Any.t -> Any.t -> R_src -> R_tgt -> iProp)
         r g f_src f_tgt st_src st_tgt
-        vaddr m q ofs tg itr_src (ktr_tgt: bool -> _)
+        vaddr m q tg itr_src (ktr_tgt: bool -> _)
         fuel0
         (STBINCL: stb_incl (to_stb MemStb) stb)
         (DEPTH: ord_lt (ord_pure 0%nat) o)
@@ -243,13 +252,13 @@ Section MEM.
     :
       bi_entails
         (inv_with le I w0 st_src st_tgt
-                  ** (⌜weak_valid m ofs⌝ ** vaddr ⊨m#q≖ (ofs, tg))
+                  ** (∃ ofs, weak_valid m vaddr ofs ** live_ q# (m, tg))
                   **
                   (∀ st_src st_tgt,
-                      ((inv_with le I w0 st_src st_tgt) ** (vaddr ⊨m#q≖ (ofs, tg))) -* isim le I mn stb o (g, g, true, true) Q (Some fuel1) (st_src, itr_src) (st_tgt, ktr_tgt true)))
+                      ((inv_with le I w0 st_src st_tgt) ** (live_ q# (m, tg))) -* isim le I mn stb o (g, g, true, true) Q (Some fuel1) (st_src, itr_src) (st_tgt, ktr_tgt true)))
         (isim le I mn stb o (r, g, f_src, f_tgt) Q (Some fuel0) (st_src, itr_src) (st_tgt, ccallU "cmp_ptr" (Cne, Vnullptr, vaddr) >>= ktr_tgt)).
   Proof.
-    iIntros "[[H0 [% H2]] H1]". iApply isim_ccallU_pure; et.
+    (* iIntros "[[H0 [% H2]] H1]". iApply isim_ccallU_pure; et.
     { eapply fn_has_spec_in_stb; et.
       { eapply STBINCL. stb_tac. ss. }
       { ss. instantiate(1:=inr (inr (inl _))).
@@ -263,7 +272,8 @@ Section MEM.
     - iIntros (st_src0 st_tgt0 ret_src ret_tgt) "H0".
       iDestruct "H0" as "[INV [[% AL] %]]".
       rewrite H4. iExists _. iSplit; et; iApply "H1"; iFrame.
-  Qed.
+  Qed. *)
+  Admitted.
 
   Lemma isim_ccallU_cmp_ptr3
         o stb w0 fuel1
@@ -278,13 +288,13 @@ Section MEM.
     :
       bi_entails
         (inv_with le I w0 st_src st_tgt
-                  ** (⌜weak_valid m ofs⌝ ** vaddr ⊨m#q≖ (ofs, tg))
+                  ** (weak_valid m vaddr ofs ** live_ q# (m, tg))
                   **
                   (∀ st_src st_tgt,
-                      ((inv_with le I w0 st_src st_tgt) ** (vaddr ⊨m#q≖ (ofs, tg))) -* isim le I mn stb o (g, g, true, true) Q (Some fuel1) (st_src, itr_src) (st_tgt, ktr_tgt false)))
+                      ((inv_with le I w0 st_src st_tgt) ** (live_ q# (m, tg))) -* isim le I mn stb o (g, g, true, true) Q (Some fuel1) (st_src, itr_src) (st_tgt, ktr_tgt false)))
         (isim le I mn stb o (r, g, f_src, f_tgt) Q (Some fuel0) (st_src, itr_src) (st_tgt, ccallU "cmp_ptr" (Ceq, vaddr, Vnullptr) >>= ktr_tgt)).
   Proof.
-    iIntros "[[H0 [% H2]] H1]". iApply isim_ccallU_pure; et.
+    (* iIntros "[[H0 [% H2]] H1]". iApply isim_ccallU_pure; et.
     { eapply fn_has_spec_in_stb; et.
       { eapply STBINCL. stb_tac. ss. }
       { ss. instantiate(1:=inr (inr (inr (inl _)))).
@@ -298,7 +308,8 @@ Section MEM.
     - iIntros (st_src0 st_tgt0 ret_src ret_tgt) "H0".
       iDestruct "H0" as "[INV [[% AL] %]]".
       rewrite H4. iExists _. iSplit; et; iApply "H1"; iFrame.
-  Qed.
+  Qed. *)
+  Admitted.
 
   Lemma isim_ccallU_cmp_ptr4
         o stb w0 fuel1
@@ -313,13 +324,13 @@ Section MEM.
     :
       bi_entails
         (inv_with le I w0 st_src st_tgt
-                  ** (⌜weak_valid m ofs⌝ ** vaddr ⊨m#q≖ (ofs, tg))
+                  ** (weak_valid m vaddr ofs ** live_ q# (m, tg))
                   **
                   (∀ st_src st_tgt,
-                      ((inv_with le I w0 st_src st_tgt) ** (vaddr ⊨m#q≖ (ofs, tg))) -* isim le I mn stb o (g, g, true, true) Q (Some fuel1) (st_src, itr_src) (st_tgt, ktr_tgt true)))
+                      ((inv_with le I w0 st_src st_tgt) ** (live_ q# (m, tg))) -* isim le I mn stb o (g, g, true, true) Q (Some fuel1) (st_src, itr_src) (st_tgt, ktr_tgt true)))
         (isim le I mn stb o (r, g, f_src, f_tgt) Q (Some fuel0) (st_src, itr_src) (st_tgt, ccallU "cmp_ptr" (Cne, vaddr, Vnullptr) >>= ktr_tgt)).
   Proof.
-    iIntros "[[H0 [% H2]] H1]". iApply isim_ccallU_pure; et.
+    (* iIntros "[[H0 [% H2]] H1]". iApply isim_ccallU_pure; et.
     { eapply fn_has_spec_in_stb; et.
       { eapply STBINCL. stb_tac. ss. }
       { ss. instantiate(1:=inr (inr (inr (inr (inl _))))).
@@ -333,14 +344,15 @@ Section MEM.
     - iIntros (st_src0 st_tgt0 ret_src ret_tgt) "H0".
       iDestruct "H0" as "[INV [[% AL] %]]".
       rewrite H4. iExists _. iSplit; et; iApply "H1"; iFrame.
-  Qed.
+  Qed. *)
+  Admitted.
 
   Lemma isim_ccallU_cmp_ptr5
         o stb w0 fuel1
         R_src R_tgt
         (Q: Any.t -> Any.t -> R_src -> R_tgt -> iProp)
         r g f_src f_tgt st_src st_tgt
-        vaddr0 vaddr1 c m ofs0 ofs1 q0 q1 tg0 tg1
+        vaddr0 vaddr1 c m ofs0 ofs1 q tg
         itr_src (ktr_tgt: bool -> _)
         fuel0
         (STBINCL: stb_incl (to_stb MemStb) stb)
@@ -349,15 +361,14 @@ Section MEM.
     :
       bi_entails
         (inv_with le I w0 st_src st_tgt
-                  ** (⌜weak_valid m ofs0 /\ weak_valid m ofs1⌝
-                      ** vaddr0 ⊨m#q0≖ (ofs0, tg0)
-                      ** vaddr1 ⊨m#q1≖ (ofs1, tg1))
+                  ** (weak_valid m vaddr0 ofs0 ** weak_valid m vaddr1 ofs1
+                      ** live_ q# (m, tg))
                   **
                   (∀ st_src st_tgt,
-                      ((inv_with le I w0 st_src st_tgt) ** (vaddr0 ⊨m#q0≖ (ofs0, tg0) ** vaddr1 ⊨m#q1≖ (ofs1, tg1))) -* isim le I mn stb o (g, g, true, true) Q (Some fuel1) (st_src, itr_src) (st_tgt, ktr_tgt (cmp_ofs c ofs0 ofs1))))
+                      ((inv_with le I w0 st_src st_tgt) ** (live_ q# (m, tg))) -* isim le I mn stb o (g, g, true, true) Q (Some fuel1) (st_src, itr_src) (st_tgt, ktr_tgt (cmp_ofs c ofs0 ofs1))))
         (isim le I mn stb o (r, g, f_src, f_tgt) Q (Some fuel0) (st_src, itr_src) (st_tgt, ccallU "cmp_ptr" (c, vaddr0, vaddr1) >>= ktr_tgt)).
   Proof.
-    iIntros "[[H0 [[% H3] H2]] H1]". des. iApply isim_ccallU_pure; et.
+    (* iIntros "[[H0 [[% H3] H2]] H1]". des. iApply isim_ccallU_pure; et.
     { eapply fn_has_spec_in_stb; et.
       { eapply STBINCL. stb_tac. ss. }
       { ss. instantiate(1:=inr (inr (inr (inr (inr (inl _)))))).
@@ -371,7 +382,8 @@ Section MEM.
     - iIntros (st_src0 st_tgt0 ret_src ret_tgt) "H0".
       iDestruct "H0" as "[INV [[[% AL'] AL] %]]".
       rewrite H5. iExists _. iSplit; et; iApply "H1"; iFrame.
-  Qed.
+  Qed. *)
+  Admitted.
 
   Lemma isim_ccallU_cmp_ptr6
         o stb w0 fuel1
@@ -387,15 +399,17 @@ Section MEM.
     :
       bi_entails
         (inv_with le I w0 st_src st_tgt
-                  ** (⌜m0 #^ m1 /\ valid m0 ofs0 /\ valid m1 ofs1⌝
-                      ** vaddr0 ⊨m0#q0≖ (ofs0, tg0)
-                      ** vaddr1 ⊨m1#q1≖ (ofs1, tg1))
+                  ** (⌜m0 #^ m1 ⌝
+                      ** valid m0 vaddr0 ofs0
+                      ** valid m1 vaddr1 ofs1
+                      ** live_ q0# (m0, tg0)
+                      ** live_ q1# (m1, tg1))
                   **
                   (∀ st_src st_tgt,
-                      ((inv_with le I w0 st_src st_tgt) ** (vaddr0 ⊨m0#q0≖ (ofs0, tg0) ** vaddr1 ⊨m1#q1≖ (ofs1, tg1))) -* isim le I mn stb o (g, g, true, true) Q (Some fuel1) (st_src, itr_src) (st_tgt, ktr_tgt false)))
+                      ((inv_with le I w0 st_src st_tgt) ** (live_ q0# (m0, tg0) ** live_ q1# (m1, tg1))) -* isim le I mn stb o (g, g, true, true) Q (Some fuel1) (st_src, itr_src) (st_tgt, ktr_tgt false)))
         (isim le I mn stb o (r, g, f_src, f_tgt) Q (Some fuel0) (st_src, itr_src) (st_tgt, ccallU "cmp_ptr" (Ceq, vaddr0, vaddr1) >>= ktr_tgt)).
   Proof.
-    iIntros "[[H0 [[% H3] H2]] H1]". iApply isim_ccallU_pure; et.
+    (* iIntros "[[H0 [[% H3] H2]] H1]". iApply isim_ccallU_pure; et.
     { eapply fn_has_spec_in_stb; et.
       { eapply STBINCL. stb_tac. ss. }
       { ss. instantiate(1:=inr (inr (inr (inr (inr (inr (inl _))))))).
@@ -408,7 +422,8 @@ Section MEM.
     - iIntros (st_src0 st_tgt0 ret_src ret_tgt) "H0".
       iDestruct "H0" as "[INV [[[% AL'] AL] %]]".
       rewrite H4. iExists _. iSplit; et; iApply "H1"; iFrame.
-  Qed.
+  Qed. *)
+  Admitted.
 
   Lemma isim_ccallU_cmp_ptr7
         o stb w0 fuel1
@@ -424,15 +439,16 @@ Section MEM.
     :
       bi_entails
         (inv_with le I w0 st_src st_tgt
-                  ** (⌜m0 #^ m1 /\ valid m0 ofs0 /\ valid m1 ofs1⌝
-                      ** vaddr0 ⊨m0#q0≖ (ofs0, tg0)
-                      ** vaddr1 ⊨m1#q1≖ (ofs1, tg1))
+                  ** (⌜m0 #^ m1 ⌝
+                      ** valid m0 vaddr0 ofs0 ** valid m1 vaddr1 ofs1
+                      ** live_ q0# (m0, tg0)
+                      ** live_ q1# (m1, tg1))
                   **
                   (∀ st_src st_tgt,
-                      ((inv_with le I w0 st_src st_tgt) ** (vaddr0 ⊨m0#q0≖ (ofs0, tg0) ** vaddr1 ⊨m1#q1≖ (ofs1, tg1))) -* isim le I mn stb o (g, g, true, true) Q (Some fuel1) (st_src, itr_src) (st_tgt, ktr_tgt true)))
+                      ((inv_with le I w0 st_src st_tgt) ** (live_ q0# (m0, tg0) ** live_ q1# (m1, tg1))) -* isim le I mn stb o (g, g, true, true) Q (Some fuel1) (st_src, itr_src) (st_tgt, ktr_tgt true)))
         (isim le I mn stb o (r, g, f_src, f_tgt) Q (Some fuel0) (st_src, itr_src) (st_tgt, ccallU "cmp_ptr" (Cne, vaddr0, vaddr1) >>= ktr_tgt)).
   Proof.
-    iIntros "[[H0 [[% H3] H2]] H1]". iApply isim_ccallU_pure; et.
+    (* iIntros "[[H0 [[% H3] H2]] H1]". iApply isim_ccallU_pure; et.
     { eapply fn_has_spec_in_stb; et.
       { eapply STBINCL. stb_tac. ss. }
       { ss. instantiate(1:=inr (inr (inr (inr (inr (inr (inr _))))))).
@@ -445,14 +461,15 @@ Section MEM.
     - iIntros (st_src0 st_tgt0 ret_src ret_tgt) "H0".
       iDestruct "H0" as "[INV [[[% AL'] AL] %]]".
       rewrite H4. iExists _. iSplit; et; iApply "H1"; iFrame.
-  Qed.
+  Qed. *)
+  Admitted.
 
   Lemma isim_ccallU_sub_ptr
         o stb w0 fuel1
         R_src R_tgt
         (Q: Any.t -> Any.t -> R_src -> R_tgt -> iProp)
         r g f_src f_tgt st_src st_tgt
-        size vaddr0 vaddr1 m ofs0 ofs1 q0 q1 tg0 tg1
+        size vaddr0 vaddr1 m ofs0 ofs1 q tg
         itr_src (ktr_tgt: val -> _)
         fuel0
         (STBINCL: stb_incl (to_stb MemStb) stb)
@@ -461,16 +478,15 @@ Section MEM.
     :
       bi_entails
         (inv_with le I w0 st_src st_tgt
-                  ** (⌜weak_valid m ofs0 /\ weak_valid m ofs1
-                      /\ (0 < size ≤ Ptrofs.max_signed)%Z⌝
-                      ** vaddr0 ⊨m#q0≖ (ofs0, tg0)
-                      ** vaddr1 ⊨m#q1≖ (ofs1, tg1))
+                  ** (⌜(0 < size ≤ Ptrofs.max_signed)%Z⌝
+                      ** weak_valid m vaddr0 ofs0 ** weak_valid m vaddr1 ofs1
+                      ** live_ q# (m, tg))
                   **
                   (∀ st_src st_tgt,
-                      ((inv_with le I w0 st_src st_tgt) ** (vaddr0 ⊨m#q0≖ (ofs0, tg0) ** vaddr1 ⊨m#q1≖ (ofs1, tg1))) -* isim le I mn stb o (g, g, true, true) Q (Some fuel1) (st_src, itr_src) (st_tgt, ktr_tgt (Vptrofs (Ptrofs.repr (Z.div (ofs0 - ofs1) size))))))
+                      ((inv_with le I w0 st_src st_tgt) ** (live_ q# (m, tg))) -* isim le I mn stb o (g, g, true, true) Q (Some fuel1) (st_src, itr_src) (st_tgt, ktr_tgt (Vptrofs (Ptrofs.repr (Z.div (ofs0 - ofs1) size))))))
         (isim le I mn stb o (r, g, f_src, f_tgt) Q (Some fuel0) (st_src, itr_src) (st_tgt, ccallU "sub_ptr" (size, vaddr0, vaddr1) >>= ktr_tgt)).
   Proof.
-    iIntros "[[H0 [[% H3] H2]] H1]". des. iApply isim_ccallU_pure; et.
+    (* iIntros "[[H0 [[% H3] H2]] H1]". des. iApply isim_ccallU_pure; et.
     { eapply fn_has_spec_in_stb; et.
       { eapply STBINCL. stb_tac. ss. }
       { ss. des_ifs. }
@@ -481,7 +497,8 @@ Section MEM.
     - iIntros (st_src0 st_tgt0 ret_src ret_tgt) "H0".
       iDestruct "H0" as "[INV [[[% AL'] AL] %]]".
       rewrite H7. iExists _. iSplit; et; iApply "H1"; iFrame.
-  Qed.
+  Qed. *)
+  Admitted.
 
   Lemma isim_ccallU_non_null
         o stb w0 fuel1
@@ -497,13 +514,13 @@ Section MEM.
     :
       bi_entails
         (inv_with le I w0 st_src st_tgt
-                  ** (⌜weak_valid m ofs⌝ ** vaddr ⊨m#q≖ (ofs, tg))
+                  ** (weak_valid m vaddr ofs ** live_ q# (m, tg))
                   **
                   (∀ st_src st_tgt,
-                      ((inv_with le I w0 st_src st_tgt) ** (vaddr ⊨m#q≖ (ofs, tg))) -* isim le I mn stb o (g, g, true, true) Q (Some fuel1) (st_src, itr_src) (st_tgt, ktr_tgt true)))
+                      ((inv_with le I w0 st_src st_tgt) ** (live_ q# (m, tg))) -* isim le I mn stb o (g, g, true, true) Q (Some fuel1) (st_src, itr_src) (st_tgt, ktr_tgt true)))
         (isim le I mn stb o (r, g, f_src, f_tgt) Q (Some fuel0) (st_src, itr_src) (st_tgt, ccallU "non_null?" vaddr >>= ktr_tgt)).
   Proof.
-    iIntros "[[H0 [% H2]] H1]". iApply isim_ccallU_pure; et.
+    (* iIntros "[[H0 [% H2]] H1]". iApply isim_ccallU_pure; et.
     { eapply fn_has_spec_in_stb; et.
       { eapply STBINCL. stb_tac. ss. }
       { ss. des_ifs. }
@@ -514,7 +531,8 @@ Section MEM.
     - iIntros (st_src0 st_tgt0 ret_src ret_tgt) "H0".
       iDestruct "H0" as "[INV [[% AL] %]]".
       rewrite H4. iExists _. iSplit; et; iApply "H1"; iFrame.
-  Qed.
+  Qed. *)
+  Admitted.
 
   Lemma isim_ccallU_malloc
         o stb w0 fuel1
@@ -532,9 +550,9 @@ Section MEM.
                   ** ⌜(Ptrofs.unsigned n > 0)%Z⌝
                   **
                   (∀ st_src st_tgt vaddr m,
-                      ((inv_with le I w0 st_src st_tgt) ** (⌜m.(sz) = Ptrofs.unsigned n⌝ ** vaddr ↦m#1≻ List.repeat Undef (Z.to_nat (Ptrofs.unsigned n)) ** vaddr ⊨m#1≖ (0, Dynamic))) -* isim le I mn stb o (g, g, true, true) Q (Some fuel1) (st_src, itr_src) (st_tgt, ktr_tgt vaddr)))
+                      ((inv_with le I w0 st_src st_tgt) ** (⌜m.(sz) = Ptrofs.unsigned n⌝ ** vaddr ↦m#1≻ List.repeat Undef (Z.to_nat (Ptrofs.unsigned n)) ** vaddr ⊨m# 0 ** live_ 1# (m, Dynamic))) -* isim le I mn stb o (g, g, true, true) Q (Some fuel1) (st_src, itr_src) (st_tgt, ktr_tgt vaddr)))
         (isim le I mn stb o (r, g, f_src, f_tgt) Q (Some fuel0) (st_src, itr_src) (st_tgt, ccallU "malloc" [Vptrofs n] >>= ktr_tgt)).
-  Proof.
+  (* Proof.
     iIntros "[[H0 %] H1]". iApply isim_ccallU_pure; et.
     { eapply fn_has_spec_in_stb; et.
       { eapply STBINCL. stb_tac. ss. }
@@ -550,7 +568,8 @@ Section MEM.
     des. clarify.
     iExists _. iSplit; ss; et.
     iApply "H1". iFrame. 
-  Qed.
+  Qed. *)
+  Admitted.
 
   Lemma isim_ccallU_mfree
         o stb w0 fuel1
@@ -565,13 +584,13 @@ Section MEM.
     :
       bi_entails
         (inv_with le I w0 st_src st_tgt
-                  ** (∃ m mvl, vaddr ↦m#1≻ mvl ** vaddr ⊨m#1≖ (0, Dynamic) ** ⌜Z.of_nat (List.length mvl) = m.(sz)⌝)
+                  ** (∃ m mvl, vaddr ↦m#1≻ mvl ** vaddr ⊨m# 0 ** live_ 1# (m, Dynamic) ** ⌜Z.of_nat (List.length mvl) = m.(sz)⌝)
                   **
                   (∀ st_src st_tgt,
                       ((inv_with le I w0 st_src st_tgt)) -* isim le I mn stb o (g, g, true, true) Q (Some fuel1) (st_src, itr_src) (st_tgt, ktr_tgt Vundef)))
         (isim le I mn stb o (r, g, f_src, f_tgt) Q (Some fuel0) (st_src, itr_src) (st_tgt, ccallU "mfree" [vaddr] >>= ktr_tgt)).
   Proof.
-    iIntros "[[H0 H2] H1]". iDestruct "H2" as (m mvl) "[[H2 H3]%]".
+    (* iIntros "[[H0 H2] H1]". iDestruct "H2" as (m mvl) "[[H2 H3]%]".
     iApply isim_ccallU_pure; et.
     { eapply fn_has_spec_in_stb; et.
       { eapply STBINCL. stb_tac. ss. }
@@ -586,7 +605,8 @@ Section MEM.
     des. clarify.
     iExists _. iSplit; ss.
     iApply "H1". iFrame. 
-  Qed.
+  Qed. *)
+  Admitted.
 
   Lemma isim_ccallU_memcpy
         o stb w0 fuel1
@@ -673,13 +693,13 @@ Section MEM.
     :
       bi_entails
         (inv_with le I w0 st_src st_tgt
-                  ** vaddr ⊨m#q≖ (ofs, tg)
+                  ** vaddr ⊨m# ofs ** live_ q# (m, tg)
                   **
                   (∀ st_src st_tgt i,
-                      (((inv_with le I w0 st_src st_tgt) ** (vaddr ⊨m#q≖ (ofs, tg) ** vaddr (≃_m) (Ptrofs.unsigned i))) -* isim le I mn stb o (g, g, true, true) Q (Some fuel1) (st_src, itr_src) (st_tgt, ktr_tgt (Vptrofs i)))))
+                      (((inv_with le I w0 st_src st_tgt) ** (live_ q# (m, tg) ** vaddr (≃_m) (Ptrofs.unsigned i))) -* isim le I mn stb o (g, g, true, true) Q (Some fuel1) (st_src, itr_src) (st_tgt, ktr_tgt (Vptrofs i)))))
         (isim le I mn stb o (r, g, f_src, f_tgt) Q (Some fuel0) (st_src, itr_src) (st_tgt, ccallU "capture" [vaddr] >>= ktr_tgt)).
   Proof.
-    iIntros "[[H0 H2] H1]". iApply isim_ccallU_pure; et.
+    (* iIntros "[[H0 H2] H1]". iApply isim_ccallU_pure; et.
     { eapply fn_has_spec_in_stb; et.
       { eapply STBINCL. stb_tac. ss. }
       { ss. instantiate (1:= inr _).
@@ -695,7 +715,8 @@ Section MEM.
     des. clarify.
     iExists _. iSplit; ss.
     iApply "H1". iSplitL "INV"; iFrame.
-  Qed.
+  Qed. *)
+  Admitted.
 
 End MEM.
 
